coq-verification/src/Concrete/Assumptions/Datatypes.v
@@ -1,3 +1,5 @@
+Require Import Hafnium.Util.List.
+
 (*** This file is for datatypes that are left abstract so as to avoid making any
      assumptions about their content. It may be necessary to instantiate these
      types later. ***)
@@ -11,3 +13,7 @@ Axiom ptable_pointer_eq_dec :
 
 (* assume NULL exists *)
 Axiom null_pointer : ptable_pointer.
+
+(* out-of-bounds accesses to lists of ptable_pointers return null_pointer *)
+Global Instance ptable_pointer_oobe : OutOfBoundsElement ptable_pointer :=
+  {| oob_value := null_pointer |}.
